Examples/division.ml
@@ -1,11 +1,9 @@
 let half (x: int) : int =
   x / 2
 [@@spec fun v ->
-  bind (isint v) @@ fun n ->
   ret (fun r ->
-    bind (isint r) @@ fun q ->
-    assert (q * 2 <= n);
-    assert (n < (q + 1) * 2))]
+    assert (r * 2 <= v);
+    assert (v < (r + 1) * 2))]
 ;;
 let _ = assert (half 10 = 5)
 ;;
